Start of proof of last lemma for soundness

DD.v
@@ -84,24 +84,19 @@ Inductive head_step_trace :
   | do_pure_step_trace e e' h b :
       pure_step_trace e e' b ->
       head_step_trace e h e' h b
-  | Newlock_head_step_trace h l :
-      l ∉ dom (gset nat) h →
-      head_step_trace
-        ENewlock h
-        (EVal (VRef l)) (<[ l := false ]> h)
-        None
   | Lock_head_step_trace h l :
-      l ∈ dom (gset nat) h ->
       head_step_trace
         (ELock (EVal (VRef l))) h
         (EVal VUnit) (<[ l := true ]> h)
         (Some (Lock l))
   | Unlock_head_step_trace h l :
-      l ∈ dom (gset nat) h ->
       head_step_trace
         (EUnlock (EVal (VRef l))) h
         (EVal VUnit) (<[ l := false ]> h)
         (Some (Unlock l)).
+
+Global Hint Constructors pure_step_trace : headstep.
+Global Hint Constructors head_step_trace : headstep.
 
 Inductive ctx_trace : (expr -> expr) -> Prop :=
   | pair_l_ctx_trace e : ctx_trace (fun x => EPair x e)
@@ -134,6 +129,18 @@ Proof.
   injection Hk; tauto.
 Qed.
 
+Lemma ctx_trace_unique e e' k k' :
+  ctx_trace k ->
+  ctx_trace k' ->
+  ¬ is_val e ->
+  ¬ is_val e' ->
+  k e = k' e' ->
+  k = k' /\ e = e'.
+Proof.
+  intros Hctx Hctx' Hnval Hnval' Heq.
+  induction Hctx; by inv Hctx'.
+Qed.
+
 Global Hint Constructors ctx_trace : context.
 Global Hint Resolve ctx_trace_ctx1 : context.
 
@@ -154,6 +161,8 @@ Inductive step_trace :
   | par_r_step_trace e1 e2 h e2' h' (b : option event) :
       step_trace e2 h e2' h' b ->
       step_trace (EPar e1 e2) h (EPar e1 e2') h' (option_map Right b).
+
+Global Hint Resolve do_head_step_trace : headstep.
 
 Lemma head_step_trace_some e h e' h' (b : base_event) :
   head_step_trace e h e' h' (Some b) ->
@@ -188,8 +197,7 @@ Proof. intros. by eapply par_r_step_trace in H. Qed.
 Lemma let_not_recursive s e1 e2 :
   ¬ e2 = ELet s e1 e2.
 Proof.
-  intros H. induction e2; try done.
-  simplify_eq.
+  intros H. induction e2; done || simplify_eq.
 Qed.
 
 Lemma step_trace_not_eq' e1 h1 e2 h2 t :
@@ -199,14 +207,24 @@ Proof.
   intros Heq Hstep.
   induction Hstep; simplify_eq.
   - inv H. inv H0.
-    + induction e; try done; simpl in H2.
+    + induction e; done || simpl in H2.
       * by destruct (string_dec s y).
       * destruct (string_dec y s); simplify_eq.
         by eapply let_not_recursive.
-    + induction e1; try done; simplify_eq.
-    + induction e2; try done; simplify_eq.
-    + induction e; try done; simplify_eq.
+    + induction e1; simplify_eq.
+    + induction e2; simplify_eq.
+    + induction e; simplify_eq.
   - eauto using ctx_trace_injective.
+Qed.
+
+Lemma step_trace_not_val e h e' h' t :
+  step_trace e h e' h' t ->
+  ¬ is_val e.
+Proof.
+  intros Hstep.
+  induction Hstep; [.. | tauto | tauto].
+  - inv H; [inv H0|..]; tauto.
+  - by apply not_is_val_ctx1, ctx_trace_ctx1.
 Qed.
 
 Lemma step_trace_not_eq e h1 h2 t :
@@ -224,6 +242,25 @@ Inductive steps_trace : expr -> lock_heap -> expr -> lock_heap -> trace -> Prop 
       step_trace e1 h1 e2 h2 (Some b) ->
       steps_trace e2 h2 e3 h3 t ->
       steps_trace e1 h1 e3 h3 (b :: t).
+
+Lemma step_trace_none_eq {e1 h1 e2 h2} :
+  step_trace e1 h1 e2 h2 None ->
+  h1 = h2.
+Proof.
+  intros Hstep. remember None as n.
+  induction Hstep; [by inv H | eauto |..];
+  destruct b; done || tauto.
+Qed.
+
+Lemma steps_trace_none_eq {e1 h1 e2 h2} :
+  steps_trace e1 h1 e2 h2 [] ->
+  h1 = h2.
+Proof.
+  intros Hstep. remember [] as t.
+  induction Hstep; [done | | done].
+  rewrite <- (IHHstep Heqt).
+  by eapply step_trace_none_eq.
+Qed.
 
 Create HintDb step_trace.
 Global Hint Constructors
@@ -247,6 +284,36 @@ Lemma step_once_some e e' h h' (b : event) :
 Proof.
   intros Hstep.
   eauto using steps_trace.
+Qed.
+
+Lemma steps_left {e1 e2 e' h h' t t'} :
+  steps_trace e1 h e2 h' t ->
+  map Left t = t' ->
+  steps_trace (EPar e1 e') h (EPar e2 e') h' t'.
+Proof.
+  intros Hsteps H. revert t' H.
+  induction Hsteps; intros t' H'.
+  - simplify_eq. simpl. constructor.
+  - eapply steps_step_none; [|eauto].
+    by apply par_l_step_trace_none.
+  - simpl in H'. simplify_eq.
+    eapply steps_step_some; [|eauto].
+    by apply par_l_step_trace_some.
+Qed.
+
+Lemma steps_right {e1 e2 e' h h' t t'} :
+  steps_trace e1 h e2 h' t ->
+  map Right t = t' ->
+  steps_trace (EPar e' e1) h (EPar e' e2) h' t'.
+Proof.
+  intros Hsteps H. revert t' H.
+  induction Hsteps; intros t' H'.
+  - simplify_eq. simpl. constructor.
+  - eapply steps_step_none; [|eauto].
+    by apply par_r_step_trace_none.
+  - simpl in H'. simplify_eq.
+    eapply steps_step_some; [|eauto].
+    by apply par_r_step_trace_some.
 Qed.
 
 Lemma steps_context_steps e e' h h' k (t : trace) :
@@ -300,122 +367,593 @@ Proof.
       by eapply steps_step_some.
 Qed.
 
+Inductive ctxs_trace : (expr -> expr) -> Prop :=
+  | Id_ctxs_trace : ctxs_trace (λ x, x)
+  | Compose_ctxs_trace k1 k2 :
+      ctx_trace k1 ->
+      ctxs_trace k2 ->
+      ctxs_trace (λ x, k1 (k2 x)).
+
+Global Hint Constructors ctxs_trace : context.
+
+Lemma ctxs_single_ctx (k : expr -> expr) :
+  ctx_trace k ->
+  ctxs_trace k.
+Proof. eauto with context. Qed.
+
+Lemma ctxs_step e1 h1 e2 h2 b k :
+  ctxs_trace k ->
+  step_trace e1 h1 e2 h2 b ->
+  step_trace (k e1) h1 (k e2) h2 b.
+Proof.
+  intros Hctx Hstep.
+  induction Hctx; by [|constructor].
+Qed.
+
+Lemma ctxs_steps {e1 h1 e2 h2 b k} :
+  ctxs_trace k ->
+  steps_trace e1 h1 e2 h2 b ->
+  steps_trace (k e1) h1 (k e2) h2 b.
+Proof.
+  intros Hctx Hsteps.
+  induction Hctx; [done|].
+  by apply steps_context_steps.
+Qed.
+
+Lemma ctx_not_val {e k} :
+  ctx_trace k ->
+  ¬ is_val (k e).
+Proof.
+  intros Hctx.
+  inv Hctx; tauto.
+Qed.
+
+Lemma ctxs_not_val {e k} :
+  ctxs_trace k ->
+  ¬ is_val e ->
+  ¬ is_val (k e).
+Proof.
+  intros Hctx Hnval.
+  inv Hctx; by [|apply ctx_not_val].
+Qed.
+
+Lemma ctx_step_not_val {e1 h1 e2 h2 b k} :
+  ctx_trace k ->
+  ¬ is_val e1 ->
+  step_trace (k e1) h1 e2 h2 b ->
+  exists e2', e2 = k e2' /\
+    step_trace e1 h1 e2' h2 b.
+Proof.
+  intros Hctx Hnval Hstep.
+  inv Hstep; [| |inv Hctx..].
+  - inv H; [|by inv Hctx..].
+    by inv H0; inv Hctx.
+  - assert (Hnval' := step_trace_not_val _ _ _ _ _ H1).
+    destruct (ctx_trace_unique _ _ _ _ H0 Hctx Hnval' Hnval H) as [-> ->].
+    eauto.
+Qed.
+
+Lemma step_left_ctxs {e1 h1 e2 h2 t} :
+  step_trace e1 h1 e2 h2 (Some (Left t)) ->
+  exists k e1' e2' e,
+    ctxs_trace k /\
+    e1 = k (EPar e1' e) /\
+    e2 = k (EPar e2' e) /\
+    step_trace e1' h1 e2' h2 (Some t).
+Proof.
+  intros Hstep. remember (Some (Left t)) as Lt.
+  induction Hstep; [by destruct b | | | by destruct b].
+  - destruct (IHHstep HeqLt) as (k0 & e1' & e2' & e0 & Hctx & -> & -> & Hstep').
+    exists (λ x, k (k0 x)), e1', e2', e0.
+    repeat split; eauto with context.
+  - destruct b; [|done]. simpl in HeqLt. simplify_eq.
+    exists (λ x, x), e1, e1', e2.
+    repeat split; eauto with context.
+Qed.
+
+Lemma step_right_ctxs {e1 h1 e2 h2 t} :
+  step_trace e1 h1 e2 h2 (Some (Right t)) ->
+  exists k e1' e2' e,
+    ctxs_trace k /\
+    e1 = k (EPar e e1') /\
+    e2 = k (EPar e e2') /\
+    step_trace e1' h1 e2' h2 (Some t).
+Proof.
+  intros Hstep. remember (Some (Right t)) as Rt.
+  induction Hstep; [by destruct b | | by destruct b |].
+  - destruct (IHHstep HeqRt) as (k0 & e1' & e2' & e0 & Hctx & -> & -> & Hstep').
+    exists (λ x, k (k0 x)), e1', e2', e0.
+    repeat split; eauto with context.
+  - destruct b; [|done]. simpl in HeqRt. simplify_eq.
+    exists (λ x, x), e2, e2', e1.
+    repeat split; eauto with context.
+Qed.
+
+Lemma step_trace_none_heap_indifferent {e h e' h'} :
+  step_trace e h e' h' None ->
+  forall h'', step_trace e h'' e' h'' None.
+Proof.
+  intros Hstep h''. remember None as t.
+  induction Hstep.
+  - constructor. destruct b; [done|simpl].
+    inv H. by constructor.
+  - constructor; tauto.
+  - constructor. destruct b; [done|tauto].
+  - apply par_r_step_trace. destruct b; [done|tauto].
+Qed.
+
+Lemma steps_trace_none_heap_indifferent {e h e' h'} :
+  steps_trace e h e' h' [] ->
+  forall h'', steps_trace e h'' e' h'' [].
+Proof.
+  intros Hsteps h''. remember [] as t.
+  induction Hsteps; [constructor | | done].
+  specialize (IHHsteps Heqt).
+  eapply steps_step_none; [|done].
+  by eapply step_trace_none_heap_indifferent.
+Qed.
+
+Lemma step_none_without_context {e1 e2 h e3} :
+  step_trace (EPar e1 e2) h e3 h None ->
+  (exists e1', e3 = (EPar e1' e2) /\ step_trace e1 h e1' h None) \/
+  (exists e2', e3 = (EPar e1 e2') /\ step_trace e2 h e2' h None).
+Proof.
+  intros Hstep.
+  inv Hstep.
+  - inv H4. inv H0.
+  - inv H0.
+  - left. exists e1'. split; [done|].
+    rewrite H5. by destruct b.
+  - right. exists e2'. split; [done|].
+    rewrite H5. by destruct b.
+Qed.
+
+Lemma step_none_in_context {e1 e2 h e3 k} :
+  ctxs_trace k ->
+  step_trace (k (EPar e1 e2)) h e3 h None ->
+  (exists e1', e3 = k (EPar e1' e2) /\ step_trace e1 h e1' h None) \/
+  (exists e2', e3 = k (EPar e1 e2') /\ step_trace e2 h e2' h None).
+Proof.
+  intros Hctx. revert e1 e2 e3 h.
+  induction Hctx; intros e1 e2 e3 h Hstep.
+  - by apply step_none_without_context.
+  - assert (Hnval : ¬ is_val (k2 (EPar e1 e2))) by (apply ctxs_not_val; tauto).
+    destruct (ctx_step_not_val H Hnval Hstep) as (e' & -> & Hstep').
+    destruct (IHHctx _ _ _ _ Hstep') as [(e1' & -> & IH) | (e2' & -> & IH)];
+    eauto.
+Qed.
+
+Lemma step_left_some_without_context {e1 e2 h1 e3 h2 t} :
+  step_trace (EPar e1 e2) h1 e3 h2 (Some (Left t)) ->
+  exists e1', e3 = EPar e1' e2 ∧ step_trace e1 h1 e1' h2 (Some t).
+Proof.
+  intros Hstep. inv Hstep.
+  - destruct b; [|done]. inv H4.
+  - inv H0.
+  - destruct b; [|done]. simpl in H5. simplify_eq. eauto.
+  - by destruct b.
+Qed.
+
+Lemma step_left_some_in_context {e1 e2 h1 e3 h2 k t} :
+  ctxs_trace k ->
+  step_trace (k (EPar e1 e2)) h1 e3 h2 (Some (Left t)) ->
+  exists e1', e3 = k (EPar e1' e2) /\ step_trace e1 h1 e1' h2 (Some t).
+Proof.
+  intros Hctx. revert e1 e2 e3 h1 h2 t.
+  induction Hctx; intros e1 e2 e3 h1 h2 t Hstep;
+  (* Case: k = λ x, x *)
+  [by apply step_left_some_without_context|].
+  (* Case: k = λ x, k1 (k2 x) *)
+  assert (Hnval : ¬ is_val (k2 (EPar e1 e2))) by (apply ctxs_not_val; tauto).
+  destruct (ctx_step_not_val H Hnval Hstep) as (e' & -> & Hstep').
+  destruct (IHHctx _ _ _ _ _ _ Hstep') as (e1' & -> & IH).
+  eauto.
+Qed.
+
+Lemma step_right_some_without_context {e1 e2 h1 e3 h2 t} :
+  step_trace (EPar e1 e2) h1 e3 h2 (Some (Right t)) ->
+  exists e2', e3 = EPar e1 e2' ∧ step_trace e2 h1 e2' h2 (Some t).
+Proof.
+  intros Hstep. inv Hstep.
+  - destruct b; [|done]. inv H4.
+  - inv H0.
+  - by destruct b.
+  - destruct b; [|done]. simpl in H5. simplify_eq. eauto.
+Qed.
+
+Lemma step_right_some_in_context {e1 e2 h1 e3 h2 k t} :
+  ctxs_trace k ->
+  step_trace (k (EPar e1 e2)) h1 e3 h2 (Some (Right t)) ->
+  exists e2', e3 = k (EPar e1 e2') /\ step_trace e2 h1 e2' h2 (Some t).
+Proof.
+  intros Hctx. revert e1 e2 e3 h1 h2 t.
+  induction Hctx; intros e1 e2 e3 h1 h2 t Hstep;
+  [by apply step_right_some_without_context|].
+  assert (Hnval : ¬ is_val (k2 (EPar e1 e2))) by (apply ctxs_not_val; tauto).
+  destruct (ctx_step_not_val H Hnval Hstep) as (e' & -> & Hstep').
+  destruct (IHHctx _ _ _ _ _ _ Hstep') as (e2' & -> & IH).
+  eauto.
+Qed.
+
+Lemma steps_left_in_context {e1 e2 h1 e3 h2 t k} :
+  ctxs_trace k ->
+  steps_trace (k (EPar e1 e2)) h1 e3 h2 [Left t] ->
+  exists e3' e2',
+    steps_trace (k (EPar e1 e2)) h1 (k (EPar e3' e2')) h2 [Left t] /\
+    steps_trace e2 h1 e2' h1 [] /\
+    steps_trace e1 h1 e3' h2 [t] /\
+    steps_trace (k (EPar e3' e2')) h2 e3 h2 [].
+Proof.
+  intros Hctx Hsteps. dependent induction Hsteps.
+  - assert (Heq := step_trace_none_eq H). subst.
+    destruct (step_none_in_context Hctx H) as [(e1' & -> & H') | (e2' & -> & H')].
+    + specialize (IHHsteps k Hctx t e2 e1' eq_refl JMeq_refl).
+      destruct IHHsteps as (e1'' & e2' & HL & HR & Ht & Hafter).
+      exists e1'', e2'. repeat split; eauto with step_trace.
+    + specialize (IHHsteps k Hctx t e2' e1 eq_refl JMeq_refl).
+      destruct IHHsteps as (e1'' & e2'' & HL & HR & Ht & Hafter).
+      exists e1'', e2''. repeat split; eauto with step_trace.
+  - assert (Heq := steps_trace_none_eq Hsteps). subst.
+    destruct (step_left_some_in_context Hctx H) as (e1' & -> & H').
+    exists e1', e2. repeat split; eauto with step_trace.
+Qed.
+
+Lemma steps_right_in_context {e1 e2 h1 e3 h2 t k} :
+  ctxs_trace k ->
+  steps_trace (k (EPar e1 e2)) h1 e3 h2 [Right t] ->
+  exists e3' e1',
+    steps_trace (k (EPar e1 e2)) h1 (k (EPar e1' e3')) h2 [Right t] /\
+    steps_trace e1 h1 e1' h1 [] /\
+    steps_trace e2 h1 e3' h2 [t] /\
+    steps_trace (k (EPar e1' e3')) h2 e3 h2 [].
+Proof.
+  intros Hctx Hsteps. dependent induction Hsteps.
+  - assert (Heq := step_trace_none_eq H). subst.
+    destruct (step_none_in_context Hctx H) as [(e1' & -> & H') | (e2' & -> & H')].
+    + specialize (IHHsteps k Hctx t e2 e1' eq_refl JMeq_refl).
+      destruct IHHsteps as (e1'' & e2' & HL & HR & Ht & Hafter).
+      exists e1'', e2'. repeat split; eauto with step_trace.
+    + specialize (IHHsteps k Hctx t e2' e1 eq_refl JMeq_refl).
+      destruct IHHsteps as (e1'' & e2'' & HL & HR & Ht & Hafter).
+      exists e1'', e2''. repeat split; eauto with step_trace.
+  - assert (Heq := steps_trace_none_eq Hsteps). subst.
+    destruct (step_right_some_in_context Hctx H) as (e2' & -> & H').
+    exists e2', e1. repeat split; eauto with step_trace.
+Qed.
+
+Lemma steps_one_split {e1 h1 e2 h2 t} :
+  steps_trace e1 h1 e2 h2 [t] ->
+  exists e1' e2',
+    steps_trace e1 h1 e1' h1 [] /\
+    step_trace e1' h1 e2' h2 (Some t) /\
+    steps_trace e2' h2 e2 h2 [].
+Proof.
+  intros Hsteps. remember [t] as tt.
+  induction Hsteps; [done|simplify_eq..].
+  - destruct (IHHsteps eq_refl) as (e1' & e2' & Hsteps1 & Hstep & Hsteps2).
+    assert (Heq := step_trace_none_eq H). subst.
+    exists e1', e2'. repeat split; try done.
+    by eapply steps_step_none.
+  - assert (Heq := steps_trace_none_eq Hsteps). subst.
+    exists e1, e2. repeat split; eauto using steps_trace.
+Qed.
+
+Lemma steps_two_split_left_right {e1 h1 e2 h2 t e3 h3 t'} :
+  step_trace e1 h1 e2 h2 (Some (Left t)) ->
+  steps_trace e2 h2 e3 h3 [Right t'] ->
+  exists e1' e2' e3',
+    steps_trace e1 h1 e1' h1 [] /\
+    step_trace e1' h1 e2' h2 (Some (Left t)) /\
+    step_trace e2' h2 e3' h3 (Some (Right t')) /\
+    steps_trace e3' h3 e3 h3 [].
+Proof.
+  intros Hstep Hsteps.
+  destruct (step_left_ctxs Hstep) as
+    (k & e1' & e1'' & e2' & Hctx & -> & -> & Hstep').
+  destruct (steps_right_in_context Hctx Hsteps) as
+    (e2'' & e1''' & Hsteps' & H1 & H2 & H3).
+  destruct (steps_one_split H2) as
+    (e2'1 & e2'2 & H2'1 & H2'2 & H2'3).
+  exists (k (EPar e1' e2'1)), (k (EPar e1'' e2'1)), (k (EPar e1'' e2'2)).
+  repeat split.
+  - apply ctxs_steps; [done|].
+    eapply steps_right; by [eapply steps_trace_none_heap_indifferent|].
+  - apply ctxs_step; [done|].
+    by apply par_l_step_trace_some.
+  - apply ctxs_step; [done|].
+    by apply par_r_step_trace_some.
+  - eapply steps_trans'.
+    + eapply ctxs_steps; [done|].
+      by eapply steps_right.
+    + eapply steps_trans'; [|done..].
+      apply ctxs_steps; [done|].
+      eapply steps_left; by [eapply steps_trace_none_heap_indifferent|].
+    + done.
+Qed.
+
+Lemma steps_two_split_right_left {e1 h1 e2 h2 t e3 h3 t'} :
+  step_trace e1 h1 e2 h2 (Some (Right t)) ->
+  steps_trace e2 h2 e3 h3 [Left t'] ->
+  exists e1' e2' e3',
+    steps_trace e1 h1 e1' h1 [] /\
+    step_trace e1' h1 e2' h2 (Some (Right t)) /\
+    step_trace e2' h2 e3' h3 (Some (Left t')) /\
+    steps_trace e3' h3 e3 h3 [].
+Proof.
+  intros Hstep Hsteps.
+  destruct (step_right_ctxs Hstep) as
+    (k & e2' & e2'' & e1' & Hctx & -> & -> & Hstep').
+  destruct (steps_left_in_context Hctx Hsteps) as
+    (e1'' & e2''' & Hsteps' & H1 & H2 & H3).
+  destruct (steps_one_split H2) as
+    (e1'1 & e1'2 & H1'1 & H1'2 & H1'3).
+  exists (k (EPar e1'1 e2')), (k (EPar e1'1 e2'')), (k (EPar e1'2 e2'')).
+  repeat split.
+  - apply ctxs_steps; [done|].
+    eapply steps_left; by [eapply steps_trace_none_heap_indifferent|].
+  - apply ctxs_step; [done|].
+    by apply par_r_step_trace_some.
+  - apply ctxs_step; [done|].
+    by apply par_l_step_trace_some.
+  - eapply steps_trans'.
+    + eapply ctxs_steps; [done|].
+      by eapply steps_left.
+    + eapply steps_trans'; [|done..].
+      apply ctxs_steps; [done|].
+      eapply steps_right; by [eapply steps_trace_none_heap_indifferent|].
+    + done.
+Qed.
+
+Lemma steps_two_split_start_some {e1 h1 e2 h2 e3 h3 x y} :
+  can_swap x y ->
+  step_trace e1 h1 e2 h2 (Some x) ->
+  steps_trace e2 h2 e3 h3 [y] ->
+  exists e1' e2' e3',
+    steps_trace e1 h1 e1' h1 [] /\
+    step_trace e1' h1 e2' h2 (Some x) /\
+    step_trace e2' h2 e3' h3 (Some y) /\
+    steps_trace e3' h3 e3 h3 [].
+Proof.
+  intros Hswap. revert e1 h1 e2 h2 e3 h3.
+  induction Hswap; intros e1 h1 e2 h2 e3 h3.
+  - (* Base case: Left Right *) apply steps_two_split_left_right.
+  - (* Base case: Right Left *) apply steps_two_split_right_left.
+  - (* Inductive case: Left Left *)
+    intros Hstep Hsteps.
+    destruct (step_left_ctxs Hstep) as
+      (k & e1' & e1'' & e2' & Hctx & -> & -> & Hstep').
+    destruct (steps_left_in_context Hctx Hsteps) as
+      (e3' & e2'' & Hctx3' & H2 & H3' & He3).
+    specialize (IHHswap e1' h1 e1'' h2 e3' h3 Hstep' H3').
+    destruct IHHswap as (ec1 & ec2 & ec3 & Hstep1 & Hstep2 & Hstep3 & Hstep4).
+    exists (k (EPar ec1 e2'')), (k (EPar ec2 e2'')), (k (EPar ec3 e2'')).
+    repeat split; eauto using ctxs_step, par_l_step_trace_some.
+    + apply ctxs_steps; [done|].
+      eapply steps_trans' with (t := []) (t' := []); [ | | done].
+      * by eapply steps_left.
+      * eapply steps_trace_none_heap_indifferent in H2.
+        by eapply steps_right.
+    + eapply steps_trans' with (t := []); [ | done | done].
+      * eapply ctxs_steps; [done|].
+        by eapply steps_left.
+  - (* Inductive case: Right Right *)
+    intros Hstep Hsteps.
+    destruct (step_right_ctxs Hstep) as
+      (k & e2' & e2'' & e1' & Hctx & -> & -> & Hstep').
+    destruct (steps_right_in_context Hctx Hsteps) as
+      (e3' & e1'' & Hctx3' & H1 & H3' & He3).
+    specialize (IHHswap e2' h1 e2'' h2 e3' h3 Hstep' H3').
+    destruct IHHswap as (ec1 & ec2 & ec3 & Hstep1 & Hstep2 & Hstep3 & Hstep4).
+    exists (k (EPar e1'' ec1)), (k (EPar e1'' ec2)), (k (EPar e1'' ec3)).
+    repeat split; eauto using ctxs_step, par_r_step_trace_some.
+    + apply ctxs_steps; [done|].
+      eapply steps_trans' with (t := []) (t' := []); [ | | done].
+      * by eapply steps_right.
+      * eapply steps_trace_none_heap_indifferent in H1.
+        by eapply steps_left.
+    + eapply steps_trans' with (t := []); [ | done | done].
+      * eapply ctxs_steps; [done|].
+        by eapply steps_right.
+Qed.
+
+Lemma steps_two_split {e h e' h' x y} :
+  can_swap x y ->
+  steps_trace e h e' h' [x; y] ->
+  exists e1 e2 h2 e3,
+    steps_trace e h e1 h [] /\
+    step_trace e1 h e2 h2 (Some x) /\
+    step_trace e2 h2 e3 h' (Some y) /\
+    steps_trace e3 h' e' h' [].
+Proof.
+  intros Hswap Hsteps.
+  remember [x;y] as xy. induction Hsteps; [done|..].
+  - simplify_eq. specialize (IHHsteps eq_refl).
+    destruct IHHsteps as (e3' & e4 & h4 & e5 & Hsteps2 & Hsteps3 & Hsteps4 & Hsteps5).
+    exists e3', e4, h4, e5.
+    assert (h1 = h2) by (by eapply step_trace_none_eq).
+    simplify_eq. repeat split; [|done..].
+    by eapply steps_step_none.
+  - simplify_eq.
+    destruct (steps_two_split_start_some Hswap H Hsteps)
+      as (e1' & e2' & e3' & Hsteps' & Hxstep & Hystep & Hsteps'').
+    by repeat eexists.
+Qed.
+
+(* Currently unused *)
+Lemma ctx_trace_step_left e h e' h' t k :
+  ctx_trace k ->
+  ¬ is_val e ->
+  step_trace (k e) h e' h' (Some (Left t)) ->
+  exists e0, e' = k e0.
+Proof.
+  intros Hctx Hnval Hstep.
+  inv Hstep; [by destruct b | .. | by destruct b].
+  - apply ctx_trace_unique in H; try done.
+    + destruct H; simplify_eq. by eexists.
+    + by eapply step_trace_not_val.
+  - inv Hctx.
+Qed.
+
+(* Currently unused *)
+Lemma ctx_trace_step_right e h e' h' t k :
+  ctx_trace k ->
+  ¬ is_val e ->
+  step_trace (k e) h e' h' (Some (Right t)) ->
+  exists e0, e' = k e0.
+Proof.
+  intros Hctx Hnval Hstep.
+  inv Hstep; try by destruct b.
+  - apply ctx_trace_unique in H; try done.
+    + destruct H; simplify_eq. by eexists.
+    + by eapply step_trace_not_val.
+  - inv Hctx.
+Qed.
+
+(* Currently unused *)
+Lemma step_left_not_val e h e' h' t :
+  step_trace e h e' h' (Some (Left t)) ->
+  ¬ is_val e'.
+Proof.
+  intros Hstep.
+  induction e'; try tauto.
+  inv Hstep.
+  - by destruct b.
+  - by apply not_is_val_ctx1, ctx_trace_ctx1.
+Qed.
+
+(* Currently unused *)
+Lemma step_right_not_val e h e' h' t :
+  step_trace e h e' h' (Some (Right t)) ->
+  ¬ is_val e'.
+Proof.
+  intros Hstep.
+  induction e'; try tauto.
+  inv Hstep.
+  - by destruct b.
+  - by apply not_is_val_ctx1, ctx_trace_ctx1.
+Qed.
+
+Lemma steps_left_map e h e' h' t t' {ek} :
+  steps_trace e h e' h' t ->
+  t' = map Left t ->
+  steps_trace (EPar e ek) h (EPar e' ek) h' t'.
+Proof.
+  intros Hsteps ->. induction Hsteps; [constructor|..].
+  - eapply steps_step_none; [|done].
+    by apply par_l_step_trace_none.
+  - eapply steps_step_some; [|done].
+    by apply par_l_step_trace_some.
+Qed.
+
+Lemma steps_right_map e h e' h' t t' {ek}:
+  steps_trace e h e' h' t ->
+  t' = map Right t ->
+  steps_trace (EPar ek e) h (EPar ek e') h' t'.
+Proof.
+  intros Hsteps ->. induction Hsteps; [constructor|..].
+  - eapply steps_step_none; [|done].
+    by apply par_r_step_trace_none.
+  - eapply steps_step_some; [|done].
+    by apply par_r_step_trace_some.
+Qed.
+
+Lemma step_trace_some_heap_indifferent h1' {e1 h1 e2 h2 b} :
+  step_trace e1 h1 e2 h2 (Some b) ->
+  exists h2', step_trace e1 h1' e2 h2' (Some b).
+Proof.
+  intros Hstep. dependent induction Hstep.
+  - destruct b0; [|done]. simpl in x.  simplify_eq.
+    inv H.
+    + inv H0. exists h1'.
+      apply head_step_trace_some. repeat constructor.
+    + eexists. apply head_step_trace_some, Lock_head_step_trace.
+    + eexists. apply head_step_trace_some, Unlock_head_step_trace.
+  - destruct (IHHstep b eq_refl) as [h2' Hstep'].
+    eexists. by constructor.
+  - destruct b0; [|done]. simpl in x. simplify_eq.
+    destruct (IHHstep e eq_refl) as [h2' Hstep'].
+    eexists. by apply par_l_step_trace_some.
+  - destruct b0; [|done]. simpl in x. simplify_eq.
+    destruct (IHHstep e eq_refl) as [h2' Hstep'].
+    eexists. by apply par_r_step_trace_some.
+Qed.
+
+Lemma step_swap {e1 h1 e2 h2 e3 h3 x y} :
+  can_swap x y ->
+  step_trace e1 h1 e2 h2 (Some x) ->
+  step_trace e2 h2 e3 h3 (Some y) ->
+  exists h', steps_trace e1 h1 e3 h' [y; x].
+Proof.
+  intros Hswap. revert e1 h1 e2 h2 e3 h3.
+  induction Hswap; intros e1 h1 e2 h2 e3 h3 Hstepx Hstepy.
+  - destruct (step_left_ctxs Hstepx) as
+      (k & e1' & e1'' & e2' & Hctx & -> & -> & Hstep1).
+    destruct (step_right_some_in_context Hctx Hstepy) as
+      (e2'' & -> & Hstep2).
+    destruct (step_trace_some_heap_indifferent h1 Hstep2) as (h2' & Hstep2').
+    destruct (step_trace_some_heap_indifferent h2' Hstep1) as (h2'' & Hstep1').
+    exists h2''. eapply steps_trans'; try apply step_once_some.
+    + apply ctxs_step; [done|].
+      by apply par_r_step_trace_some.
+    + apply ctxs_step; [done|].
+      by apply par_l_step_trace_some.
+    + done.
+  - destruct (step_right_ctxs Hstepx) as
+      (k & e2' & e2'' & e1' & Hctx & -> & -> & Hstep1).
+    destruct (step_left_some_in_context Hctx Hstepy) as
+      (e1'' & -> & Hstep2).
+    destruct (step_trace_some_heap_indifferent h1 Hstep2) as (h2' & Hstep2').
+    destruct (step_trace_some_heap_indifferent h2' Hstep1) as (h2'' & Hstep1').
+    exists h2''. eapply steps_trans'; try apply step_once_some.
+    + apply ctxs_step; [done|].
+      by apply par_l_step_trace_some.
+    + apply ctxs_step; [done|].
+      by apply par_r_step_trace_some.
+    + done.
+  - destruct (step_left_ctxs Hstepx) as
+      (k & e1' & e1'' & e2' & Hctx & -> & -> & Hstep1).
+    destruct (step_left_some_in_context Hctx Hstepy) as
+      (e1''' & -> & Hstep2).
+    destruct (IHHswap _ _ _ _ _ _ Hstep1 Hstep2) as [h' Hsteps].
+    exists h'. apply ctxs_steps; [done|].
+    by eapply steps_left_map.
+  - destruct (step_right_ctxs Hstepx) as
+      (k & e2' & e2'' & e1' & Hctx & -> & -> & Hstep1).
+    destruct (step_right_some_in_context Hctx Hstepy) as
+      (e2''' & -> & Hstep2).
+    destruct (IHHswap _ _ _ _ _ _ Hstep1 Hstep2) as [h' Hsteps].
+    exists h'. apply ctxs_steps; [done|].
+    by eapply steps_right_map.
+Qed.
+
 Lemma steps_swap {e h e' h' x y} :
   can_swap x y ->
   steps_trace e h e' h' [y; x] ->
   exists h'', steps_trace e h e' h'' [x; y].
-Proof. Admitted.
-(* steps_swap is false, since the following program doesn't allow swaps *)
-
-Definition steps_swap_false l l' :=
-  (EPar (ELock (EVal (VRef l'))) (ESeq (ELock (EVal (VRef l))) (ENewlock))).
-
-Check ({[ 0 := false; 1 := false]}) : lock_heap.
-
-Lemma contradiction : False.
 Proof.
-  assert (
-    steps_trace
-      (steps_swap_false 0 1) {[0 := false]}
-      (EPar (EVal VUnit) (EVal (VRef 1))) {[1 := true; 0 := true]}
-      [Right (Base (Lock 0)); Left (Base (Lock 1))]).
-  { unfold steps_swap_false. eapply steps_step_some. {
-    apply par_r_step_trace_some.
-    apply ctx_step_trace with (k := fun x => ESeq x _); eauto with context.
-    apply head_step_trace_some.
-    by constructor. } rewrite insert_singleton.
-    eapply steps_step_none. {
-    apply par_r_step_trace_none, head_step_trace_none. repeat constructor. }
-    eapply steps_step_none. {
-    apply par_r_step_trace_none, head_step_trace_none.
-    by apply Newlock_head_step_trace with (l := 1). }
-    eapply steps_step_some. {
-    apply par_l_step_trace_some, head_step_trace_some.
-    by constructor. } rewrite insert_insert. apply steps_refl_trace.
-  } unfold steps_swap_false in H.
-  apply steps_swap in H; [|constructor].
-  destruct H as [h'' H]. inv H.
-  - inv H0.
-    + inv H6. inv H0.
-    + inv H2.
-    + inv H6.
-      * inv H. inv H0.
-      * inv H0. inv H2.
-        -- inv H. inv H0.
-        -- inv H0.
-    + inv H6.
-      * inv H. inv H0.
-      * inv H0. inv H2.
-        -- inv H. inv H0.
-        -- inv H0. inv H3.
-           ++ inv H. inv H0.
-           ++ inv H0.
-  - inv H6.
-    + inv H4. inv H0.
-    + inv H0.
-    + inv H4.
-      * inv H.
-        -- inv H0.
-        -- discriminate. (* The crucial step *)
-      * inv H0. inv H1.
-        -- inv H. inv H0.
-        -- inv H0.
-    + destruct b; done.
+  intros Hswap Hsteps.
+  apply can_swap_symm in Hswap.
+  destruct (steps_two_split Hswap Hsteps) as
+    (e1 & e2 & h2 & e3 & Hsteps1 & Hstepy & Hstepx & Hsteps2).
+  destruct (step_swap Hswap Hstepy Hstepx) as [hi Hstepsxy].
+  eapply steps_trace_none_heap_indifferent in Hsteps2.
+  exists hi. eauto using steps_trans'.
 Qed.
 
-Lemma step_trace_heap_indifferent {e1 h1 h1' e2 h2 t} :
-  dom (gset nat) h1 = dom (gset nat) h1' ->
-  step_trace e1 h1 e2 h2 t ->
-  exists h2', step_trace e1 h1' e2 h2' t.
+Lemma steps_trace_heap_indifferent h1' {e1 h1 e2 h2 t} :
+  steps_trace e1 h1 e2 h2 t ->
+  exists h2', steps_trace e1 h1' e2 h2' t.
 Proof.
-  intros Hdom Hstep.
-  induction Hstep.
-  - inversion H; [|rewrite Hdom in H0..]; simplify_eq.
-    + exists h1'. by do 2 constructor.
-    + eexists. constructor. by apply Newlock_head_step_trace.
-    + eexists. constructor. by apply Lock_head_step_trace.
-    + eexists. constructor. by apply Unlock_head_step_trace.
-  - destruct (IHHstep Hdom) as [h2' IH].
-    eexists; by constructor.
-  - destruct (IHHstep Hdom) as [h2' IH].
-    eexists; by constructor.
-  - destruct (IHHstep Hdom) as [h2' IH].
-    eexists; by constructor.
-Qed.
-
-Lemma step_trace_dom_eq {e0 h0 e1 h1 h1' t t'} :
-  steps_trace e0 h0 e1 h1 t ->
-  steps_trace e0 h0 e1 h1' t' ->
-  dom (gset nat) h1 = dom (gset nat) h1'.
-Proof. Admitted.
-
-Lemma steps_trace_heap_indifferent {e0 h0 e1 h1 h1' e2 h2 t0 t0' t1} :
-  steps_trace e0 h0 e1 h1 t0 ->
-  steps_trace e0 h0 e1 h1' t0' ->
-  steps_trace e1 h1 e2 h2 t1 ->
-  exists h2', steps_trace e1 h1' e2 h2' t1.
-Proof.
-  intros Hsteps1 Hsteps1' Hsteps2.
-  revert e0 h0 h1' t0 t0' Hsteps1 Hsteps1'.
-  induction Hsteps2;
-  intros e0 h0 h1' t0 t0' Hsteps1 Hsteps1'.
+  intros Hsteps. revert h1'.
+  induction Hsteps; intros h1'.
   - exists h1'. constructor.
-  - assert (dom (gset nat) h1 = dom (gset nat) h1');
-    [by eapply step_trace_dom_eq|].
-    destruct (step_trace_heap_indifferent H0 H) as [h2' H'].
-    destruct (IHHsteps2 e0 h0 h2' (t0 ++ []) (t0' ++ [])) as [h3' Hsteps3].
-    + eapply steps_trans; [done|]. by apply step_once_none.
-    + eapply steps_trans; [done|]. by apply step_once_none.
-    + exists h3'. replace t with ([] ++ t) by reflexivity.
-      eapply steps_trans; [|done]. by apply step_once_none.
-  - assert (dom (gset nat) h1 = dom (gset nat) h1');
-    [by eapply step_trace_dom_eq|].
-    destruct (step_trace_heap_indifferent H0 H) as [h2' H'].
-    edestruct (IHHsteps2 e0 h0 h2') as [h3' Hsteps3].
-    + eapply steps_trans; [apply Hsteps1|]. by apply step_once_some.
-    + eapply steps_trans; [done|]. by apply step_once_some.
-    + exists h3'. replace (b :: t) with ([b] ++ t) by reflexivity.
-      eapply steps_trans; [|done]. by apply step_once_some.
+  - destruct (IHHsteps h1') as [h3' Hsteps'].
+    exists h3'. eapply steps_step_none; [|done].
+    by eapply step_trace_none_heap_indifferent.
+  - apply (step_trace_some_heap_indifferent h1') in H.
+    destruct H as [h2' Hstep2].
+    destruct (IHHsteps h2') as [h3' Hsteps3].
+    eexists. by eapply steps_step_some.
 Qed.
 
 Lemma steps_perm e h e' h' (t t' : trace) :
@@ -438,7 +976,9 @@ Proof.
     replace (x :: y :: t') with ([x; y] ++ t') by reflexivity.
     destruct (steps_split _ _ _ _ _ _ Hsteps) as (e1 & h1 & Hsteps1 & Hsteps2).
     destruct (steps_swap Hswap Hsteps1) as [h1' Hsteps1'].
-    destruct (steps_trace_heap_indifferent Hsteps1 Hsteps1' Hsteps2) as (h3 & Hsteps3).
+    assert (Hperm : perm [y; x] [x; y]).
+    { constructor. constructor. by apply can_swap_symm. }
+    destruct (steps_trace_heap_indifferent h1' Hsteps2) as (h3 & Hsteps3).
     destruct (IH _ _ _ _ Hsteps3) as (h4 & Hsteps4).
     exists h4. by eapply steps_trans.
   - intros t t' t'' Hperm IH Hperm' IH' e h e' h' Hsteps.
@@ -446,23 +986,6 @@ Proof.
     edestruct IH'; [done|].
     by eexists.
 Qed.
-
-Check perm_ind_bis.
-
-Fixpoint to_base (e : event) : base_event :=
-  match e with
-  | Base b => b
-  | Left b => to_base b
-  | Right b => to_base b
-  end.
-
-Lemma left_to_base_eq (e : event) :
-  to_base (Left e) = to_base e.
-Proof. done. Qed.
-
-Lemma right_to_base_eq (e : event) :
-  to_base (Right e) = to_base e.
-Proof. done. Qed.
 
 (* The proof of this theorem uses that gen_tree, from stdpp, is Countable *)
 Global Instance val_countable : Countable val.
@@ -491,6 +1014,21 @@ Proof.
   refine (inj_countable' enc dec _). intros.
   induction x; eauto. simpl. by f_equal.
 Qed.
+
+Fixpoint to_base (e : event) : base_event :=
+  match e with
+  | Base b => b
+  | Left b => to_base b
+  | Right b => to_base b
+  end.
+
+Lemma left_to_base_eq (e : event) :
+  to_base (Left e) = to_base e.
+Proof. done. Qed.
+
+Lemma right_to_base_eq (e : event) :
+  to_base (Right e) = to_base e.
+Proof. done. Qed.
 
 (* alocks are the active locks, the locks that are currently locked *)
 Fixpoint alocks_stateful (p : trace) (a : gset nat) : gset nat :=
@@ -555,6 +1093,26 @@ Fixpoint next_events_stateful
 Definition next_events (p : trace) : gset base_event :=
   next_events_stateful p ∅ ∅.
 
+Lemma subset_next_events_stateful p n u :
+  n ⊆ next_events_stateful p n u.
+Proof.
+  revert n u.
+  induction p; [done|]; intros n u. simpl.
+  destruct (decide (set_Exists (is_parent_or_child (thread a)) u)).
+  - apply IHp.
+  - etransitivity; [|apply IHp]. set_solver.
+Qed.
+
+Lemma next_events_head b t :
+  to_base b ∈ next_events (b :: t).
+Proof.
+  unfold next_events. simpl.
+  destruct (decide (set_Exists (is_parent_or_child (thread b)) ∅));
+  [by apply set_Exists_empty in s|].
+  simpl. eapply elem_of_weaken; [|apply subset_next_events_stateful].
+  set_solver.
+Qed.
+
 (* Checks wether, given a list of active locks, a base event is locking,
    meaning that a Lock instruction is trying to get a lock that is locked,
    or that an Unlock instruction is trying to release a lock that is unlocked *)
@@ -565,6 +1123,7 @@ Definition is_locking (al : gset nat) (e : base_event) : Prop :=
   | Join => False
   end.
 
+(* Currently unused *)
 Lemma forall_is_locking_empty (t : list base_event) :
   Forall (is_locking ∅) t ->
   Forall (fun e => exists l, e = Unlock l) t.
@@ -629,6 +1188,7 @@ Lemma valid_to_base_cons_iff b t a :
   valid_stateful (b :: t) a <-> valid_stateful (Base (to_base b) :: t) a.
 Proof. split; intros; done. Qed.
 
+(* Currently only used in unused lemmas *)
 Lemma valid_stateful_is_locking t b a :
   valid_stateful t a ->
   valid_stateful (t ++ [b]) a \/ is_locking (alocks_stateful t a) (to_base b).
@@ -643,6 +1203,7 @@ Proof.
     simpl; tauto.
 Qed.
 
+(* Currently unused *)
 Lemma valid_is_locking t b :
   valid t ->
   valid (t ++ [b]) \/ is_locking (alocks t) (to_base b).
@@ -679,7 +1240,7 @@ Lemma step_trace_none_step (e e' : expr) h h' :
 Proof.
   intros Hstep. remember None as n.
   induction Hstep; destruct b; try done.
-  - apply head_step_step. inv H; [|by constructor].
+  - apply head_step_step. inv H.
     apply do_pure_step.
     inv H0; by constructor.
   - apply step_context_step;
@@ -748,16 +1309,18 @@ Proof.
     + inv H0. eauto with headstep.
     + apply do_step with (k := fun x => x); eauto with context.
       constructor. rewrite valid_to_base_iff in Hvalid.
-      rewrite <- H0 in Hvalid. destruct Hvalid as [Hvalid _].
-      rewrite elem_of_dom in H5. destruct H5. destruct x; [|done].
+      rewrite <- H5 in Hvalid. destruct Hvalid as [Hvalid _].
       rewrite not_elem_of_dom in Hvalid.
       rewrite map_filter_lookup_None in Hvalid.
-      destruct Hvalid as [Hnone | Hfalse]; [simplify_eq|].
-      specialize (Hfalse true H). done.
+      destruct Hvalid as [Hnone | Hfalse].
+      * left. by rewrite not_elem_of_dom.
+      * simpl in Hfalse. destruct (h !! l) eqn:H.
+        -- right. destruct b0; [|done].
+           by specialize (Hfalse true eq_refl).
+        -- left. by rewrite not_elem_of_dom.
     + apply do_step with (k := fun x => x); eauto with context.
       constructor. rewrite valid_to_base_iff in Hvalid.
-      rewrite <- H0 in Hvalid. destruct Hvalid as [Hvalid _].
-      rewrite elem_of_dom in H5. destruct H5. destruct x; [done|].
+      rewrite <- H5 in Hvalid. destruct Hvalid as [Hvalid _].
       rewrite elem_of_dom in Hvalid.
       destruct Hvalid as [x Hvalid].
       apply map_filter_lookup_Some_1_2 in Hvalid as Hv.
@@ -774,11 +1337,7 @@ Lemma step_trace_heap_locks_none e1 h1 e2 h2:
 Proof.
   intros Hsteps. remember None as n.
   induction Hsteps; [ | | destruct b; [done|]..]; eauto.
-  destruct b; [done|]. inv H; [done|].
-  unfold heap_locks.
-  rewrite map_filter_insert_False; [|done].
-  rewrite delete_notin; [done|].
-  by rewrite not_elem_of_dom in H0.
+  destruct b; [done|]. by inv H.
 Qed.
 
 Lemma heap_locks_lock l h :
@@ -809,8 +1368,8 @@ Proof.
   simplify_eq. inv H; [|simpl in Hvalid..].
   - inv H0. rewrite valid_to_base_cons_iff in Hvalid.
     by rewrite <- H3 in Hvalid.
-  - rewrite <- H0 in Hvalid. rewrite heap_locks_lock; tauto.
-  - rewrite <- H0 in Hvalid. rewrite heap_locks_unlock; tauto.
+  - rewrite <- H5 in Hvalid. rewrite heap_locks_lock; tauto.
+  - rewrite <- H5 in Hvalid. rewrite heap_locks_unlock; tauto.
 Qed.
 
 Lemma steps_trace_valid_steps (e e' : expr) h h' t :
@@ -852,9 +1411,9 @@ Proof.
   induction Hstep; [|tauto..].
   simplify_eq. inv H.
   - inv H0. simpl. by rewrite <- H3.
-  - simpl. rewrite <- H0.
+  - simpl. rewrite <- H5.
     by rewrite heap_locks_lock.
-  - simpl. rewrite <- H0.
+  - simpl. rewrite <- H5.
     by rewrite heap_locks_unlock.
 Qed.
 
@@ -869,9 +1428,9 @@ Proof.
   induction Hstep; [|tauto..].
   simplify_eq. inv H.
   - inv H0. simpl in Hvalid. by rewrite <- H3 in Hvalid.
-  - simpl in Hvalid. rewrite <- H0 in Hvalid.
+  - simpl in Hvalid. rewrite <- H5 in Hvalid.
     rewrite heap_locks_lock. tauto.
-  - simpl in Hvalid. rewrite <- H0 in Hvalid.
+  - simpl in Hvalid. rewrite <- H5 in Hvalid.
     rewrite heap_locks_unlock. tauto.
 Qed.
 
@@ -899,16 +1458,312 @@ Proof.
   by rewrite heap_locks_empty.
 Qed.
 
-Definition next_threads (t : trace) : gset (list bool).
-Admitted. (* Idea: Redefine next_events in terms of next_threads *)
-
-Lemma next_events_app t t' n n' u :
-  next_events t = n ->
-  next_threads t = u ->
-  next_events_stateful t' n u = n' ->
-  next_events (t ++ t') = n'.
+Lemma not_step_trace_val {v h1 e h2 t} :
+  ¬ step_trace (EVal v) h1 e h2 t.
 Proof.
+  intros Hstep. inv Hstep.
+  - inv H. inv H0.
+  - inv H0.
+Qed.
+
+Ltac unique_tac := repeat
+  match goal with
+  | H : ctx_trace _ |- _ => inv H
+  | H : step_trace (EVal _) _ _ _ _ |- _ => by apply not_step_trace_val in H
+  | H : pure_step_trace _ _ _ |- _ => inv H
+  | H : head_step_trace _ _ _ _ _ |- _ => inv H
+  | H : step_trace _ _ _ _ _ |- _ => inv H
+  | _ => intros || reflexivity
+  end.
+
+Lemma head_step_trace_unique {e1 h1 e2 h2 b} :
+  head_step_trace e1 h1 e2 h2 b ->
+  forall e' h' t, step_trace e1 h1 e' h' t -> t = option_map Base b.
+Proof. unique_tac. Qed.
+
+Lemma par_base_is_join {e1 e2 h1 e h2 b} :
+  step_trace (EPar e1 e2) h1 e h2 (Some (Base b)) ->
+  b = Join.
+Proof.
+  intros Hstep. inv Hstep.
+  - destruct b0; [|done]. simpl in H. simplify_eq.
+    inv H4. by inv H.
+  - inv H0.
+  - by destruct b0.
+  - by destruct b0.
+Qed.
+
+Lemma join_in_trace_par {e1 e2 h1 v h2 t} :
+  steps_trace (EPar e1 e2) h1 (EVal v) h2 t ->
+  (Base Join) ∈ t.
+Proof.
+  intros Hsteps. remember (EVal v) as ev.
+  remember (EPar e1 e2) as ep. revert e1 e2 Heqep.
+  induction Hsteps; intros e1' e2' Heq; simplify_eq.
+  - assert (Heq := step_trace_none_eq H). subst.
+    destruct (step_none_without_context H) as
+      [(? & -> & _) | (? & -> & _)]; eauto.
+  - destruct b; [|apply elem_of_list_further..].
+    + apply par_base_is_join in H. subst. apply elem_of_list_here.
+    + destruct (step_left_some_without_context H) as (e & -> & _). eauto.
+    + destruct (step_right_some_without_context H) as (e & -> & _). eauto.
+Qed.
+
+Lemma is_val_decision e : Decision (is_val e).
+Proof. destruct e; (right; progress eauto) || by left. Qed.
+
+Lemma steps_none_in_context {e h v k} :
+  ctx_trace k ->
+  steps_trace (k e) h (EVal v) h [] ->
+  exists v', steps_trace e h (EVal v') h [].
+Proof.
+  intros Hctx Hsteps.
+  remember (k e) as ke. revert e Heqke.
+  remember (EVal v) as ev. remember [] as t.
+  induction Hsteps; intros e' Heqke; [inv Hctx | subst | done].
+  destruct (is_val_decision e') as [Hval | Hnval].
+  - destruct e'; simpl in Hval; [|done..].
+    eauto using steps_trace.
+  - destruct (ctx_step_not_val Hctx Hnval H) as (e'' & -> & He'').
+    destruct (IHHsteps eq_refl eq_refl e'' eq_refl) as [v' Hv'].
+    assert (Heq := steps_trace_none_eq Hsteps). subst.
+    assert (Heq := step_trace_none_eq He''). subst.
+    eauto using steps_trace.
+Qed.
+
+Lemma steps_trace_singleton_unique {e1 h1 e2 h2 b v h3} :
+  step_trace e1 h1 e2 h2 (Some b) ->
+  steps_trace e2 h2 (EVal v) h3 [] ->
+  forall e' h' t, step_trace e1 h1 e' h' t -> t = Some b.
+Proof.
+  intros Hstep. revert v.
+  remember (Some b) as t.
+  induction Hstep; intros v Hsteps.
+  - by eapply head_step_trace_unique.
+  - assert (Heq := steps_trace_none_eq Hsteps). subst.
+    destruct (steps_none_in_context H Hsteps) as [v' Hv'].
+    intros e1 h1 b1 H1. apply step_trace_not_val in Hstep.
+    destruct (ctx_step_not_val H Hstep H1) as (e1' & -> & He1').
+    eauto.
+  - by apply join_in_trace_par, not_elem_of_nil in Hsteps.
+  - by apply join_in_trace_par, not_elem_of_nil in Hsteps.
+Qed.
+
+Lemma step_trace_heap_indifferent {e1 h1 e2 h2 b h1'} :
+  step_trace e1 h1 e2 h2 b ->
+  exists h2', step_trace e1 h1' e2 h2' b.
+Proof.
+  intros Hstep. destruct b.
+  - by eapply step_trace_some_heap_indifferent.
+  - eapply step_trace_none_heap_indifferent in Hstep.
+    eauto.
+Qed.
+
+Lemma step_trace_event_postponed {e1 h1 e2 h2 b e2' h2' b'} :
+  step_trace e1 h1 e2 h2 b ->
+  step_trace e1 h1 e2' h2' b' -> 
+  b ≠ b' ->
+  exists e3 h3, step_trace e2' h2' e3 h3 b.
+Proof.
+  intros Hstep Hstep' Hne. revert e2 h2 b Hstep Hne.
+  induction Hstep'; intros e'' h'' b' Hstep Hne.
+  - by eapply head_step_trace_unique in H.
+  - apply step_trace_not_val in Hstep'.
+    destruct (ctx_step_not_val H Hstep' Hstep) as (e2 & -> & H2).
+    destruct (IHHstep' _ _ _ H2 Hne) as (e3 & h3 & H3).
+    eauto using step_trace.
+  - inv Hstep.
+    + inv H. inv H0. by apply step_trace_not_val in Hstep'.
+    + inv H0.
+    + destruct b0; destruct b; simpl in Hne; [..|done];
+      destruct (IHHstep' _ _ _ H5) as (? & ? & ?);
+      eauto using step_trace. intros Heq. simplify_eq.
+    + eapply step_trace_heap_indifferent in H5.
+      destruct H5 as [h2' H5]. eauto using step_trace.
+  - inv Hstep.
+    + inv H. inv H0. by apply step_trace_not_val in Hstep'.
+    + inv H0.
+    + eapply step_trace_heap_indifferent in H5.
+      destruct H5 as [h2' H5]. eauto using step_trace.
+    + destruct b0; destruct b; simpl in Hne; [..|done];
+      destruct (IHHstep' _ _ _ H5) as (? & ? & ?);
+      eauto using step_trace. intros Heq. simplify_eq.
+Qed.
+
+Lemma steps_trace_in_trace {e1 h1 v h2 t} :
+  steps_trace e1 h1 (EVal v) h2 t ->
+  forall e' h' b, step_trace e1 h1 e' h' (Some b) ->
+  In b t.
+Proof.
+  intros Hsteps. remember (EVal v) as ev.
+  induction Hsteps; subst.
+  - intros e' h' b Hstep. by apply not_step_trace_val in Hstep.
+    (* Is this lemma even useful? *)
 Admitted.
+
+Lemma step_trace_in_next_events_stateful {e1 h1 e2 h2 v h3 t t' n u} :
+  steps_trace e1 h1 e2 h2 t ->
+  t ≠ [] ->
+  next_events t = next_events_stateful [] n u ->
+  steps_trace e2 h2 (EVal v) h3 t' ->
+  t' ≠ [] ->
+  forall e' h' b', step_trace e1 h1 e' h' (Some b') ->
+  to_base b' ∈ next_events_stateful t' n u.
+Proof.
+  intros Hsteps1 Hne Hnext Hsteps2.
+  remember (EVal v) as ev.
+  revert e1 h1 t n u Hne Hsteps1 Hnext.
+  induction Hsteps2; intros e0 h0 t0 n u Hne Hsteps1 Hnext Hne'; subst; [done|..].
+  - apply (IHHsteps2 eq_refl _ _ _ _ _ Hne); [|done..].
+    eapply steps_trans'; [done | by apply step_once_none |].
+    apply app_nil_r.
+  - destruct t; intros e' h' b' Hstep'.
+    + simpl. destruct (decide (set_Exists (is_parent_or_child (thread b)) u)).
+      * remember Hnext as Hnext2.  simpl in Hnext. rewrite <- Hnext.
+        clear IHHsteps2 Hne' HeqHnext2. admit.
+      * rewrite elem_of_union elem_of_singleton. admit.
+    + 
+Admitted. (* simpl in Hnext. rewrite <- Hnext. intros e' h' b' Hstep'.
+    eapply elem_of_weaken; [|apply subset_next_events_stateful].
+    apply (steps_trace_in_trace Hsteps1 _ _ _) in Hstep'.
+    destruct Hstep'; [subst|done].
+    apply next_events_head.
+  - eapply (IHHsteps2 eq_refl); [|done].
+    eapply steps_trans'; by [ | apply step_once_none | ].
+  - simpl. destruct (decide (set_Exists (is_parent_or_child (thread b)) u)).
+    (* Impossible? *)
+Admitted. *)
+
+(* Lemma used directly in steps_trace_heap_locks_stuck *)
+Lemma step_trace_in_next_events {e h1 v h2 t} :
+  steps_trace e h1 (EVal v) h2 t ->
+  forall e' h' b, step_trace e h1 e' h' (Some b) ->
+  to_base b ∈ next_events t.
+Proof.
+  intros Hsteps. remember (EVal v) as ev. induction Hsteps.
+  - intros ??? H. subst. by apply not_step_trace_val in H.
+  - intros e' h' b Hstep.
+    destruct (step_trace_event_postponed Hstep H) as
+      (e3' & h3' & Hstep'); eauto.
+  - subst. destruct t; intros e' h' b' Hstep'.
+    + eapply steps_trace_singleton_unique in Hstep';
+      [| apply H | eauto using steps_trace]. simplify_eq.
+      apply next_events_head.
+    + admit.
+Admitted.
+
+Lemma steps_trace_none_first_some {e1 h1 e2 h2 e3 v h3 b t} :
+  step_trace e1 h1 e2 h2 (Some b) ->
+  steps_trace e2 h2 e3 h2 [] ->
+  steps_trace e3 h2 (EVal v) h3 t ->
+  (forall e' h' t', step_trace e3 h2 e' h' t' -> exists b', t' = Some b') ->
+  exists e',
+    steps_trace e1 h1 e' h1 [] /\
+    steps_trace e' h1 (EVal v) h3 (b :: t) /\
+    forall e'' h'' t', step_trace e' h1 e'' h'' t' ->
+      exists b', t' = Some b'.
+Proof.
+  intros Hstep Hnone Hrest Hin.
+  induction Hnone.
+  - exists e1. repeat split; [eauto using steps_trace..|]. admit.
+  - 
+Admitted.
+
+Lemma steps_trace_none_first {e h v h' pt} :
+  steps_trace e h (EVal v) h' pt ->
+  pt ≠ [] ->
+  exists e',
+    steps_trace e h e' h [] /\
+    steps_trace e' h (EVal v) h' pt /\
+    (forall e'' h'' t,
+      step_trace e' h e'' h'' t -> exists b, t = Some b).
+Proof.
+  intros Hsteps Hpt. remember (EVal v) as ev.
+  induction Hsteps; subst; [done | | destruct t]; [| clear IHHsteps Hpt |].
+  - (* Case: None step *)
+    specialize (IHHsteps eq_refl Hpt).
+    destruct IHHsteps as (e' & Hnone & Hrest & Hin).
+    assert (Heq := step_trace_none_eq H). subst.
+    exists e'. repeat split; eauto using steps_trace.
+  - (* Case: Some step, t = [] *)
+    assert (Hunique := steps_trace_singleton_unique H Hsteps).
+    exists e1. repeat split; eauto using steps_trace.
+  - (* Case: Some step, t ≠ [] *)
+    destruct IHHsteps as (e' & Hnone & Hrest & Hin); [done..|].
+      (* Proof idea: split Hnone into two steps:
+        1) Steps that can be done before (H : step_trace e1 h1 e2 h2 (Some b))
+        2) Steps that can only be done after that step
+       Then the order of steps will be (1) H (2) Hrest
+       which completes the proof *)
+    (* May need some lemmas about next_events *)
+    by eapply steps_trace_none_first_some.
+Qed.
+
+Lemma steps_trace_not_val {e h e' h' t} :
+  steps_trace e h e' h' t ->
+  t ≠ [] ->
+  ¬ is_val e.
+Proof.
+  intros Hsteps Ht.
+  inv Hsteps; by eapply step_trace_not_val.
+Qed.
+
+Lemma head_step_to_step_trace {e h e' h'} :
+  head_step e h e' h' ->
+  exists t,
+    step_trace e h e' h' t /\
+    forall b, t = Some b -> ¬ is_locking (heap_locks h) (to_base b).
+Proof.
+  intros Hstep. inv Hstep.
+  - inv H; [exists (option_map Base None); split;
+      try done; eauto with headstep..|].
+    exists (option_map Base (Some Join)). split; [eauto with headstep|].
+    simpl. intros b Heq Hlock. by simplify_eq.
+  - eexists. split; [eauto with headstep|].
+    simpl. intros b Heq Hlock. simplify_eq.
+    simpl in Hlock. destruct H as [Hnelem | Hfalse].
+    * eapply Hnelem, elem_of_weaken; [done|].
+      apply dom_filter_subseteq.
+    * rewrite elem_of_dom in Hlock.
+      destruct Hlock as [x Hlock].
+      apply map_filter_lookup_Some_1_2 in Hlock as Hl. simpl in Hl.
+      apply map_filter_lookup_Some_1_1 in Hlock. simplify_eq.
+  - eexists. split; [eauto with headstep|].
+    simpl. intros b Heq Hlock. simplify_eq.
+    simpl in Hlock. rewrite not_elem_of_dom in Hlock.
+    rewrite map_filter_lookup_None in Hlock.
+    destruct Hlock as [? | Hlock]; [simplify_eq | by eapply Hlock].
+Qed.
+
+Lemma step_to_step_trace {e h e' h'} :
+  step e h e' h' ->
+  exists t,
+    step_trace e h e' h' t /\
+    forall b, t = Some b ->
+      ¬ is_locking (heap_locks h) (to_base b).
+Proof.
+  intros Hstep. inv Hstep.
+  induction H; [by apply head_step_to_step_trace|].
+  destruct IHctx as (t & Hstep & Hlock).
+  inv H; try by (exists t; split; try apply Hlock;
+    apply ctx_step_trace; eauto with context).
+  - exists t. split; [|apply Hlock].
+    apply ctx_step_trace with (k := fun x => EPair x e); eauto with context.
+  - exists t. split; [|apply Hlock].
+    apply ctx_step_trace with (k := fun x => ELet y x e); eauto with context.
+  - exists t. split; [|apply Hlock].
+    apply ctx_step_trace with (k := fun x => EOp op x e); eauto with context.
+  - exists t. split; [|apply Hlock].
+    apply ctx_step_trace with (k := fun x => EIf x e1 e2); eauto with context.
+  - exists t. split; [|apply Hlock].
+    apply ctx_step_trace with (k := fun x => ESeq x e); eauto with context.
+  - exists (option_map Left t). split; [by constructor|].
+    intros b Heq Hb. destruct t; [|done]. simpl in Heq.
+    simplify_eq. by eapply Hlock.
+  - exists (option_map Right t). split; [by constructor|].
+    intros b Heq Hb. destruct t; [|done]. simpl in Heq.
+    simplify_eq. by eapply Hlock.
+Qed.
 
 Lemma steps_trace_heap_locks_stuck e h v h' pt :
   steps_trace e h (EVal v) h' pt ->
@@ -916,9 +1771,18 @@ Lemma steps_trace_heap_locks_stuck e h v h' pt :
   set_Forall (is_locking (heap_locks h)) (next_events pt) ->
   stuck e h.
 Proof.
-  (* Need to generalize to next_events_stateful *)
-  (* Idea: Need some lemma about imm_stuck *)
-Admitted.
+  intros Hsteps Hpt Hlock.
+  destruct (steps_trace_none_first Hsteps Hpt) as
+    (e' & Hnone & Hrest & Hin).
+  exists e', h. repeat split.
+  - by eapply steps_trace_valid_steps.
+  - by eapply steps_trace_not_val.
+  - intros e'' h'' Hstep.
+    destruct (step_to_step_trace Hstep) as (t & Hstept & Ht).
+    destruct (Hin _ _ _ Hstept) as [b ->].
+    apply (step_trace_in_next_events Hrest) in Hstept.
+    by apply (Ht b eq_refl), Hlock.
+Qed.
 
 Theorem trace_soundness (e : expr) (v : val) h' (t : trace) :
   steps_trace e ∅ (EVal v) h' t ->
@@ -930,7 +1794,7 @@ Proof.
   destruct Hsteps as [h1 Hsteps].
   apply (steps_split _ _ _ _ _ _) in Hsteps as (e' & h'' & Hsteps & Hsteps').
   eapply steps_trace_stuck; [|rewrite heap_locks_empty|]; [done..|].
-  erewrite steps_trace_locks in Hdeadlock; try done.
+  erewrite steps_trace_locks in Hdeadlock; [|done..].
   by eapply steps_trace_heap_locks_stuck.
 Qed.
 
